cryptis/lib/dh.v
@@ -29,6 +29,7 @@ Definition dh_seed t : iProp :=
   minted t ∧
   □ (public t ↔ ▷ False) ∧
   □ (∀ t', exp_pred_base t t' ↔ ▷ □ dh_publ t') ∧
+  □ (public (TInv t) ↔ ▷ False) ∧
   □ (∀ t', exp_pred_base (TInv t) t' ↔ ▷ False).
 
 Lemma dh_seed_elim0 a :
@@ -120,12 +121,12 @@ Lemma dh_public_TExp g a :
   ▷ □ P (TExp g a) -∗
   public (TExp g a).
 Proof.
-iIntros "%gXN #gP (#m & #aP1 & #aP2 & _) #P_a".
+iIntros "%gXN #gP (#m & #aP1 & #aP2 & #aPV & _) #P_a".
 rewrite public_TExp_iff //; do !iSplit => //.
 - iApply exp_pred_intro1. iApply "aP2"; do 2!iModIntro; iSplit => //.
   by rewrite exps_TExpN exps_expN.
 - iModIntro; iIntros "#p".
-  by iApply False_public; last iApply "aP1".
+  by iApply False_public; last iApply "aPV".
 Qed.
 
 Definition mk_dh : val := mk_nonce.
@@ -144,25 +145,33 @@ Lemma wp_mk_dh (T : gset term) g (Ψ : val → iProp) :
   WP mk_dh #() {{ Ψ }}.
 Proof.
 iIntros "% #ctx #minted_g #minted_T post".
+iApply wp_fupd.
 iApply (wp_mk_nonce_freshN T (λ _, False%I) dh_publ
-         (λ t, {[t; TExp g t]})
+         (λ t, {[t; TInv t; TExp g t]})
   with "[//]" ) => //.
   iIntros "%t".
   rewrite big_sepS_forall; iIntros (t').
-  rewrite elem_of_union !elem_of_singleton; iIntros "[->|->]"; eauto.
-  rewrite minted_TExp //; iIntros "!>"; iSplit; eauto.
-  by iIntros "[??]".
-iIntros (a) "%a_T %nonce_a #m_a #aP #? #? token".
+  rewrite !elem_of_union !elem_of_singleton; iIntros "[[->|->]|->]"; eauto.
+  - by rewrite minted_TInv; iIntros "!>"; iSplit; eauto.
+  - rewrite minted_TExp //; iIntros "!>"; iSplit; eauto.
+    by iIntros "[??]".
+iIntros (a) "%a_T %nonce_a #m_a #aP #? #sV #? token".
 have a_g: TInv a ∉ exps g.
   by rewrite exps_expN // elem_of_nil; case.
-have [? a_ga] := tsize_lt_TExp a_g.
+have [? [] aV_ga a_ga] := tsize_lt_TExp a_g.
+have {}a_aV : TInv a ≠ a := @TInv_neq a.
 have {}a_ga : a ≠ TExp g a.
   move=> contra; rewrite -contra in a_ga; lia.
+have {}aV_ga : TInv a ≠ TExp g a.
+  move=> contra; rewrite -contra in aV_ga; lia.
 rewrite big_sepS_union ?big_sepS_singleton; last set_solver.
-rewrite bi.intuitionistic_intuitionistically.
-iDestruct "token" as "[t1 t2]".
+iDestruct "token" as "[t1 t3]".
+rewrite big_sepS_union ?big_sepS_singleton; last set_solver.
+iDestruct "t1" as "[t1 t2]".
+iMod ("sV" $! False%I with "t2") as "#s2V" => //.
 iApply ("post" with "[//] [] [$] [$]") => //.
-  by rewrite /dh_seed; do 4!iSplit => //.
+  iFrame "#"; rewrite bi.intuitionistic_intuitionistically.
+  by eauto.
 iPureIntro => t t' t_T t'_t; split => contra.
 - apply: (a_T _ t_T); congruence.
 - rewrite -[t']TInvK -contra in t'_t.
