cryptis/primitives/with_cryptis.v
@@ -196,6 +196,7 @@ Lemma twp_mk_nonce_freshN (T : gset term) (P Q : term → iProp Σ) (T' : term �
         minted t -∗
         □ (public t ↔ ▷ □ P t) -∗
         □ (∀ t', exp_pred_base t t' ↔ ▷ □ Q t') -∗
+        □ (∀ P, term_token (TInv t) ⊤ ==∗ □ (public (TInv t) ↔ ▷ □ P)) -∗
         □ (∀ t', exp_pred_base (TInv t) t' ↔ ▷ False) -∗
         ([∗ set] t' ∈ T' t, term_token t' ⊤) -∗
         Ψ t) -∗
@@ -231,8 +232,10 @@ iApply (twp_mk_nonce_gen P Q ⊤ _
     + by iDestruct "fresh" as "[_ >fresh]".
   iFrame. do !iModIntro.
   iDestruct "post" as "(? & ? & ?)". eauto. }
-iIntros "% ? ? ? ? ? [? ?]".
-iApply ("post" with "[$] [$] [$] [$] [$] [$] [$]").
+iIntros "%a %nonce_a #ma ? ? ? [? ?]".
+iApply ("post" with "[$] [//] [$] [$] [$] [] [$] [$]").
+iIntros "!> %R token".
+iMod (public_TInv_alloc R with "token") as "[??]" => //; by case: a nonce_a.
 Qed.
 
 Lemma wp_mk_nonce_freshN (T : gset term) P Q (T' : term → gset term) Ψ :
@@ -244,6 +247,7 @@ Lemma wp_mk_nonce_freshN (T : gset term) P Q (T' : term → gset term) Ψ :
         minted t -∗
         □ (public t ↔ ▷ □ P t) -∗
         □ (∀ t', exp_pred_base t t' ↔ ▷ □ Q t') -∗
+        □ (∀ P, term_token (TInv t) ⊤ ==∗ □ (public (TInv t) ↔ ▷ □ P)) -∗
         □ (∀ t', exp_pred_base (TInv t) t' ↔ ▷ False) -∗
         ([∗ set] t' ∈ T' t, term_token t' ⊤) -∗
         Ψ t) -∗
@@ -261,6 +265,7 @@ Lemma twp_mk_nonce_fresh (T : gset term) (P Q : term → iProp Σ) Ψ :
         minted t -∗
         □ (public t ↔ ▷ □ P t) -∗
         □ (∀ t', exp_pred_base t t' ↔ ▷ □ Q t') -∗
+        □ (∀ P, term_token (TInv t) ⊤ ==∗ □ (public (TInv t) ↔ ▷ □ P)) -∗
         □ (∀ t', exp_pred_base (TInv t) t' ↔ ▷ False) -∗
         term_token t ⊤ -∗
         Ψ t) -∗
@@ -284,6 +289,7 @@ Lemma wp_mk_nonce_fresh (T : gset term) P Q Ψ :
         minted t -∗
         □ (public t ↔ ▷ □ P t) -∗
         □ (∀ t', exp_pred_base t t' ↔ ▷ □ Q t') -∗
+        □ (∀ P, term_token (TInv t) ⊤ ==∗ □ (public (TInv t) ↔ ▷ □ P)) -∗
         □ (∀ t', exp_pred_base (TInv t) t' ↔ ▷ False) -∗
         term_token t ⊤ -∗
         Ψ t) -∗
@@ -299,6 +305,7 @@ Lemma twp_mk_nonce (P Q : term → iProp Σ) Ψ :
         minted t -∗
         □ (public t ↔ ▷ □ P t) -∗
         □ (∀ t', exp_pred_base t t' ↔ ▷ □ Q t') -∗
+        □ (∀ P, term_token (TInv t) ⊤ ==∗ □ (public (TInv t) ↔ ▷ □ P)) -∗
         □ (∀ t', exp_pred_base (TInv t) t' ↔ ▷ False) -∗
         term_token t ⊤ -∗
         Ψ t) -∗
@@ -315,6 +322,7 @@ Lemma wp_mk_nonce (P Q : term → iProp Σ) Ψ :
         minted t -∗
         □ (public t ↔ ▷ □ P t) -∗
         □ (∀ t', exp_pred_base t t' ↔ ▷ □ Q t') -∗
+        □ (∀ P, term_token (TInv t) ⊤ ==∗ □ (public (TInv t) ↔ ▷ □ P)) -∗
         □ (∀ t', exp_pred_base (TInv t) t' ↔ ▷ False) -∗
         term_token t ⊤ -∗
         Ψ t) -∗
@@ -341,7 +349,7 @@ iApply (twp_mk_nonce_freshN ∅ (λ _, shot γ 1) (λ _, False%I)
 - iIntros "% ?". by rewrite elem_of_empty.
 - iIntros "%t". rewrite [term_of_aenc_key]unlock big_sepS_singleton minted_TKey.
   iModIntro. by iSplit; iIntros "?".
-iIntros "%t %fresh % #m_t #s_t _ _ token".
+iIntros "%t %fresh % #m_t #s_t _ _ _ token".
 rewrite big_sepS_singleton.
 pose sk := AEncKey t.
 iAssert (public sk ↔ ▷ □ shot γ 1)%I as "s_sk".
@@ -383,7 +391,7 @@ iApply (twp_mk_nonce_freshN ∅ (λ _, shot γ 1) (λ _, False%I)
 - iIntros "% ?". by rewrite elem_of_empty.
 - iIntros "%t". rewrite [term_of_sign_key]unlock big_sepS_singleton minted_TKey.
   iModIntro. by iSplit; iIntros "?".
-iIntros "%t %fresh % #m_t #s_t _ _ token".
+iIntros "%t %fresh % #m_t #s_t _ _ _ token".
 rewrite big_sepS_singleton.
 pose sk := SignKey t.
 iAssert (public sk ↔ ▷ □ shot γ 1)%I as "s_sk".
@@ -425,7 +433,7 @@ iApply (twp_mk_nonce_freshN ∅ (λ _, shot γ 1) (λ _, False%I)
 - iIntros "% ?". by rewrite elem_of_empty.
 - iIntros "%t". rewrite [term_of_senc_key]unlock big_sepS_singleton minted_TKey.
   iModIntro. by iSplit; iIntros "?".
-iIntros "%t %fresh % #m_t #s_t _ _ token".
+iIntros "%t %fresh % #m_t #s_t _ _ _ token".
 rewrite big_sepS_singleton.
 pose sk := SEncKey t.
 iAssert (public sk ↔ ▷ □ shot γ 1)%I as "s_sk".
