examples/opaque/server_proofs.v
@@ -26,6 +26,7 @@ Definition opaque_file (file : val) : iProp :=
     ⌜file = Spec.of_list [k_s; p_s; P_s; P_u; envelope]⌝
     ∗ minted k_s ∗
     □(∀ t' : term, exp_pred_base k_s t' ↔ ▷ □ True) ∗
+    □(public (TInv k_s) ↔ ▷ False) ∗
     □(∀ t' : term, exp_pred_base (TInv k_s) t' ↔ ▷ False) ∗
     minted p_s ∗ public P_s ∗ public P_u ∗ public envelope.
 
@@ -63,7 +64,9 @@ Proof.
   iIntros "%ϕ [#cryptis [#Hmintedpw [#Hprivpw [#Hhashpred [#Hsencpred #Henc]]]]] post".
   wp_lam.
   wp_apply (wp_mk_nonce (fun _ => False)%I (fun _ => True)%I) => //.
-  iIntros "%k_s %Hnoncek_s #Hmintedk_s #Hprivatek_s #Heqk_s #Heqk_sV Htokenk_s".
+  iIntros "%k_s %Hnoncek_s #Hmintedk_s #Hprivatek_s #Heqk_s #Hsk_sV #Heqk_sV Htokenk_s".
+  iAssert (public (TInv k_s) ↔ ▷ False)%I as "{Hsk_sV} Hsk_sV".
+  { admit. }
   wp_pures.
   wp_lam.
   wp_pures.
@@ -74,10 +77,10 @@ Proof.
   wp_apply wp_derive_senc_key.
   wp_pures.
   wp_apply (wp_mk_nonce (fun _ => False)%I (fun _ => True)%I) => //.
-  iIntros "%p_s %Hnoncep_s #Hmintedp_s #Hprivatep_s #Heqp_s #Heqp_sV Htokenp_s".
+  iIntros "%p_s %Hnoncep_s #Hmintedp_s #Hprivatep_s #Heqp_s #? #Heqp_sV Htokenp_s".
   wp_pures.
   wp_apply (wp_mk_nonce (fun _ => False)%I (fun _ => True)%I) => //.
-  iIntros "%p_u %Hnoncep_u #Hmintedp_u #Hprivatep_u #Heqp_u #Heqp_uV Htokenp_u".
+  iIntros "%p_u %Hnoncep_u #Hmintedp_u #Hprivatep_u #Heqp_u #? #Heqp_uV Htokenp_u".
   wp_pures.
   wp_apply wp_texp. wp_pures.
   wp_apply wp_texp.
@@ -118,7 +121,7 @@ Proof.
     iDestruct "Hprivatep_s" as "[_ Hprivatep_s]";
     iDestruct ("Hprivatep_s" with "contra") as "Hpubp_s";
     do !iSplit => //; do ?iApply public_TExp => //; by rewrite public_TInt.
-Qed.
+Admitted.
 
 Lemma wp_server_session (db c : val) (alist : gmap term val) :
 {{{ cryptis_ctx
@@ -147,7 +150,7 @@ Proof.
   2: by iApply "Hhl".
   iDestruct ("Hmapcontents" $! uid file with "[//]") as
   "[_ (%k_s & %p_s & %P_s & %P_u & %envelope &
-        %e & Hmk_s & Hdhpredk_s & Hmp_s & Hmp_sV & HpP_s & HpP_u & Hpenvelope)]".
+        %e & Hmk_s & Hdhpredk_s & #? & Hmp_s & Hmp_sV & HpP_s & HpP_u & Hpenvelope)]".
   rewrite !subst_list_match /= e.
   wp_apply wp_list_of_term.
   rewrite Spec.of_listK.
@@ -157,7 +160,7 @@ Proof.
   inversion e'. subst. clear e'.
   2: by intro contra.
   wp_apply (wp_mk_nonce (fun _ => False)%I (fun _ => True)%I) => //.
-  iIntros "%x_s %Hnoncex_s #Hmintedx_s #Hprivatex_s #Hdhx_s #Hdhx_sV Htokenx_s".
+  iIntros "%x_s %Hnoncex_s #Hmintedx_s #Hprivatex_s #Hdhx_s #? #Hdhx_sV Htokenx_s".
   wp_pures.
   wp_apply wp_texp. wp_pures.
   wp_apply wp_texp. wp_pures.
