examples/pk_auth/nsl.v
@@ -64,7 +64,7 @@ Next Obligation.
 iIntros "%skI %skR % %Φ [#? _] post". rewrite /nsl_mk_key_share_impl.
 wp_pures. wp_bind (mk_nonce _).
 iApply (wp_mk_nonce (λ _, corruption skI skR) (λ _, False)%I) => //.
-iIntros "%n % #s_n #p_n _ _ token". wp_pures. iModIntro.
+iIntros "%n % #s_n #p_n _ _ _ token". wp_pures. iModIntro.
 iApply "post". rewrite bi.intuitionistic_intuitionistically. by eauto.
 Qed.
 
